Add lemmas about common patterns of memory accesses
Also add some assumptions that we will have to prove as invariants, e.g.
that the limit of available capabilities is smaller or equal to 2^64.

CHERI_Lemmas.thy
@@ -328,6 +328,22 @@ lemma translate_address_aligned32_plus16:
   find_theorems (70) "(_ + _) mod _"
   sorry
 
+lemma AArch64_MemSingle_read_translate_address_Some:
+  assumes "Run (AArch64_MemSingle_read vaddr sz acctype wasaligned) t a"
+    and "trace_assms t"
+  shows "\<exists>paddr. translate_address (unat vaddr) = Some paddr"
+  using assms
+  unfolding AArch64_MemSingle_read_def AArch64_TranslateAddress_def
+  by (auto elim!: Run_bindE simp: exp_fails_if_then_else IsFault_def translate_correct)
+
+lemma AArch64_MemSingle_set_translate_address_Some:
+  assumes "Run (AArch64_MemSingle_set vaddr sz acctype wasaligned data) t a"
+    and "trace_assms t"
+  shows "\<exists>paddr. translate_address (unat vaddr) = Some paddr"
+  using assms
+  unfolding AArch64_MemSingle_set_def AArch64_TranslateAddress_def
+  by (auto elim!: Run_bindE simp: exp_fails_if_then_else IsFault_def translate_correct)
+
 (* TODO *)
 (*lemma
   assumes "load_enabled s (vaddr + offset) acctype sz tagged"
@@ -349,7 +365,7 @@ lemma perm_bits_included_refl[simp, intro]:
   "perm_bits_included p p"
   by (auto simp: perm_bits_included_def)
 
-lemma perm_bits_included_OR[intro]:
+lemma perm_bits_included_OR[simp, intro]:
   assumes "perm_bits_included p p1 \<or> perm_bits_included p p2"
   shows "perm_bits_included p (p1 OR p2)"
   using assms
@@ -468,6 +484,12 @@ proof -
     by auto
 qed
 
+lemma AArch64_CheckAlignment_ATOMICRW_aligned[simp]:
+  assumes "Run (AArch64_CheckAlignment addr (int sz) AccType_ATOMICRW iswrite) t a" and "sz > 0"
+  shows "aligned (unat addr) sz"
+  using assms
+  by (auto simp: AArch64_CheckAlignment_def elim!: Run_bindE Run_letE Run_ifE)
+
 lemma TranslateAddress_aligned_vaddr_aligned_paddr:
   assumes "Run (AArch64_TranslateAddressWithTag vaddr acctype iswrite wasaligned sz iscapwrite) t addrdesc"
     and "FaultRecord_statuscode (AddressDescriptor_fault addrdesc) = Fault_None"
@@ -495,7 +517,7 @@ lemma CheckCapabilityAlignment_address_tag_aligned[intro, simp]:
 
 lemma CapIsTagClear_iff_not_128th[simp]:
   "CapIsTagClear c \<longleftrightarrow> \<not>CapIsTagSet c"
-  by (auto simp: CapIsTagClear_def CapGetTag_def CAP_TAG_BIT_def nth_ucast test_bit_of_bl)
+  by (auto simp: CapIsTagClear_def CapGetTag_def nth_ucast test_bit_of_bl)
 
 lemma more_CC_simps[simp]:
   "is_sealed_method CC c = CapIsSealed c"
@@ -725,9 +747,26 @@ lemma return_prod_snd_derivable_caps[derivable_capsE]:
   using assms
   by auto
 
-lemma VADeref_load_enabled[derivable_capsE]:
+lemma VADeref_addr_l2p64[intro, simp, derivable_capsE]:
   assumes "Run (VADeref va sz perms acctype) t vaddr" "trace_assms t"
-    and "nat sz \<le> 2^64" and "unat vaddr \<le> vaddr'" and "vaddr' + nat sz' \<le> unat vaddr + nat sz"
+  shows "uint vaddr + sz \<le> 2^64"
+  (* TODO: Add capability validness assumption to trace_assms, and prove
+     that it is an invariant of the derivable caps *)
+  sorry
+
+lemma VADeref_addr_l2p64_nat[intro, simp, derivable_capsE]:
+  assumes "Run (VADeref va sz perms acctype) t vaddr" "trace_assms t"
+    and "0 \<le> sz"
+  shows "unat vaddr + nat sz \<le> 2^64"
+  using VADeref_addr_l2p64[OF assms(1,2)] assms(3)
+  by (auto simp add: unat_def simp flip: nat_add_distrib)
+
+text \<open>Loads enabled by VADeref\<close>
+
+lemma VADeref_load_enabled:
+  assumes "Run (VADeref va sz perms acctype) t vaddr" "trace_assms t"
+    and "0 \<le> sz"
+    and "unat vaddr + nat sz \<le> 2^64 \<longrightarrow> unat vaddr \<le> vaddr' \<and> vaddr' + nat sz' \<le> unat vaddr + nat sz"
     and "perm_bits_included CAP_PERM_LOAD perms"
     and "tagged \<longrightarrow> perm_bits_included CAP_PERM_LOAD_CAP perms"
     and "tagged \<longrightarrow> nat sz' = 16 \<and> aligned vaddr' 16"
@@ -736,32 +775,182 @@ lemma VADeref_load_enabled[derivable_capsE]:
   shows "load_enabled (run s t) vaddr' sz' tagged"
   using assms(1,2)
   unfolding VADeref_def
-  by - (derivable_capsI assms: assms(3-) elim: CheckCapability_load_enabled)
+  by - (derivable_capsI assms: assms(3-) VADeref_addr_l2p64_nat[OF assms(1,2)]
+                        elim: CheckCapability_load_enabled)
+
+text \<open>Common patterns\<close>
+
+lemma VADeref_data_load_enabled[derivable_capsE]:
+  assumes "Run (VADeref va sz CAP_PERM_LOAD acctype) t vaddr" "trace_assms t"
+    and "0 \<le> sz"
+    and "unat vaddr + nat sz \<le> 2^64 \<longrightarrow> unat vaddr \<le> vaddr' \<and> vaddr' + nat sz' \<le> unat vaddr + nat sz"
+    and "VA_derivable va s"
+    and "{''PCC''} \<subseteq> accessible_regs s"
+  shows "load_enabled (run s t) vaddr' sz' False"
+  using assms
+  by (elim VADeref_load_enabled) auto
+
+lemma VADeref_data_load_enabled'[derivable_capsE]:
+  assumes "Run (VADeref va sz (CAP_PERM_LOAD OR perms) acctype) t vaddr" "trace_assms t"
+    and "0 \<le> sz"
+    and "unat vaddr + nat sz \<le> 2^64 \<longrightarrow> unat vaddr \<le> vaddr' \<and> vaddr' + nat sz' \<le> unat vaddr + nat sz"
+    and "VA_derivable va s"
+    and "{''PCC''} \<subseteq> accessible_regs s"
+  shows "load_enabled (run s t) vaddr' sz' False"
+  using assms
+  by (elim VADeref_load_enabled) auto
+
+lemma VADeref_cap_load_enabled[derivable_capsE]:
+  assumes "Run (VADeref va sz (or_vec CAP_PERM_LOAD CAP_PERM_LOAD_CAP) acctype) t vaddr" "trace_assms t"
+    and "0 \<le> sz"
+    and "unat vaddr + nat sz \<le> 2^64 \<longrightarrow> unat vaddr \<le> vaddr' \<and> vaddr' + nat sz' \<le> unat vaddr + nat sz"
+    and "nat sz' = 16 \<and> aligned vaddr' 16"
+    and "VA_derivable va s"
+    and "{''PCC''} \<subseteq> accessible_regs s"
+  shows "load_enabled (run s t) vaddr' sz' True"
+  using assms
+  by (elim VADeref_load_enabled) auto
+
+lemma VADeref_cap_load_enabled'[derivable_capsE]:
+  assumes "Run (VADeref va sz (or_vec CAP_PERM_LOAD CAP_PERM_LOAD_CAP OR perms) acctype) t vaddr" "trace_assms t"
+    and "0 \<le> sz"
+    and "unat vaddr + nat sz \<le> 2^64 \<longrightarrow> unat vaddr \<le> vaddr' \<and> vaddr' + nat sz' \<le> unat vaddr + nat sz"
+    and "nat sz' = 16 \<and> aligned vaddr' 16"
+    and "VA_derivable va s"
+    and "{''PCC''} \<subseteq> accessible_regs s"
+  shows "load_enabled (run s t) vaddr' sz' True"
+  using assms
+  by (elim VADeref_load_enabled) auto
+
+lemma VADeref_load_data_access_enabled'[derivable_capsE]:
+  assumes "Run (VADeref va sz (CAP_PERM_LOAD OR perms) acctype) t vaddr" "trace_assms t"
+    and "0 \<le> sz"
+    and "translate_address (unat vaddr) = Some paddr"
+    and "VA_derivable va s"
+    and "{''PCC''} \<subseteq> accessible_regs s"
+  shows "\<exists>vaddr. access_enabled (run s t) Load vaddr paddr (nat sz) data B0"
+  using assms
+  by (auto intro: VADeref_data_load_enabled')
+
+text \<open>Stores enabled by VADeref\<close>
+
+lemma VADeref_store_enabled:
+  assumes "Run (VADeref va sz perms acctype) t vaddr" "trace_assms t"
+    and "0 \<le> sz"
+    and "unat vaddr + nat sz \<le> 2^64 \<longrightarrow> unat vaddr \<le> vaddr' \<and> vaddr' + nat sz' \<le> unat vaddr + nat sz"
+    and "perm_bits_included CAP_PERM_STORE perms"
+    and "tag \<longrightarrow> perm_bits_included CAP_PERM_STORE_CAP perms"
+    and "tag \<and> CapIsLocal (Capability_of_tag_word tag (ucast data)) \<longrightarrow> perm_bits_included CAP_PERM_STORE_LOCAL perms"
+    and "tag \<longrightarrow> LENGTH('a) = 128 \<and> nat sz' = 16 \<and> aligned vaddr' 16"
+    and "VA_derivable va s"
+    and "{''PCC''} \<subseteq> accessible_regs s"
+  shows "store_enabled (run s t) vaddr' sz' (data :: 'a::len word) tag"
+  using assms(1,2)
+  unfolding VADeref_def
+  by - (derivable_capsI assms: assms(3-) VADeref_addr_l2p64_nat[OF assms(1,2)]
+                        elim: CheckCapability_store_enabled)
+
+text \<open>Common patterns\<close>
 
 lemma VADeref_store_data_enabled[derivable_capsE]:
-  assumes "Run (VADeref va sz perms acctype) t vaddr" "trace_assms t"
-    and "nat sz \<le> 2^64" and "unat vaddr \<le> vaddr'" and "vaddr' + nat sz' \<le> unat vaddr + nat sz"
-    and "perm_bits_included CAP_PERM_STORE perms"
+  assumes "Run (VADeref va sz CAP_PERM_STORE acctype) t vaddr" "trace_assms t"
+    and "0 \<le> sz"
+    and "unat vaddr + nat sz \<le> 2^64 \<longrightarrow> unat vaddr \<le> vaddr' \<and> vaddr' + nat sz' \<le> unat vaddr + nat sz"
     and "VA_derivable va s"
     and "{''PCC''} \<subseteq> accessible_regs s"
   shows "store_enabled (run s t) vaddr' sz' (data :: 'a::len word) False"
-  using assms(1,2)
-  unfolding VADeref_def
-  by - (derivable_capsI assms: assms(3-) elim: CheckCapability_store_enabled)
+  using assms
+  by (elim VADeref_store_enabled) auto
 
-lemma VADeref_store_enabled[derivable_capsE]:
-  assumes "Run (VADeref va sz perms acctype) t vaddr" "trace_assms t"
-    and "nat sz \<le> 2^64" and "unat vaddr \<le> vaddr'" and "vaddr' + nat sz' \<le> unat vaddr + nat sz"
-    and "perm_bits_included CAP_PERM_STORE perms"
-    and "tag \<longrightarrow> perm_bits_included CAP_PERM_STORE_CAP perms"
-    and "tag \<and> CapIsLocal (Capability_of_tag_word tag data) \<longrightarrow> perm_bits_included CAP_PERM_STORE_LOCAL perms"
-    and "tag \<longrightarrow> nat sz' = 16 \<and> aligned vaddr' 16"
+lemma VADeref_store_data_enabled'[derivable_capsE]:
+  assumes "Run (VADeref va sz (perms OR CAP_PERM_STORE) acctype) t vaddr" "trace_assms t"
+    and "0 \<le> sz"
+    and "unat vaddr + nat sz \<le> 2^64 \<longrightarrow> unat vaddr \<le> vaddr' \<and> vaddr' + nat sz' \<le> unat vaddr + nat sz"
     and "VA_derivable va s"
     and "{''PCC''} \<subseteq> accessible_regs s"
-  shows "store_enabled (run s t) vaddr' sz' data tag"
-  using assms(1,2)
-  unfolding VADeref_def
-  by - (derivable_capsI assms: assms(3-) elim: CheckCapability_store_enabled)
+  shows "store_enabled (run s t) vaddr' sz' (data :: 'a::len word) False"
+  using assms
+  by (elim VADeref_store_enabled) auto
+
+abbreviation cap_store_perms where
+  "cap_store_perms c \<equiv>
+     (if CapIsLocal c \<and> CapIsTagSet c then
+        or_vec (or_vec CAP_PERM_STORE CAP_PERM_STORE_CAP) CAP_PERM_STORE_LOCAL
+      else
+        or_vec CAP_PERM_STORE CAP_PERM_STORE_CAP)"
+
+lemma VADeref_store_cap_enabled[derivable_capsE]:
+  assumes "Run (VADeref va sz (cap_store_perms c) acctype) t vaddr" "trace_assms t"
+    and "0 \<le> sz"
+    and "unat vaddr + nat sz \<le> 2^64 \<longrightarrow> unat vaddr \<le> vaddr' \<and> vaddr' + 16 \<le> unat vaddr + nat sz"
+    and "aligned vaddr' 16"
+    and "Capability_of_tag_word tag data = c"
+    and "VA_derivable va s"
+    and "{''PCC''} \<subseteq> accessible_regs s"
+  shows "store_enabled (run s t) vaddr' 16 (data :: 128 word) tag"
+  using assms
+  by (elim VADeref_store_enabled) (auto split: if_splits)
+
+lemma VADeref_store_cap_enabled'[derivable_capsE]:
+  assumes "Run (VADeref va sz (perms OR cap_store_perms c) acctype) t vaddr" "trace_assms t"
+    and "0 \<le> sz"
+    and "unat vaddr + nat sz \<le> 2^64 \<longrightarrow> unat vaddr \<le> vaddr' \<and> vaddr' + 16 \<le> unat vaddr + nat sz"
+    and "aligned vaddr' 16"
+    and "Capability_of_tag_word tag data = c"
+    and "VA_derivable va s"
+    and "{''PCC''} \<subseteq> accessible_regs s"
+  shows "store_enabled (run s t) vaddr' 16 (data :: 128 word) tag"
+  using assms
+  by (elim VADeref_store_enabled) (auto split: if_splits)
+
+lemma VADeref_store_data_access_enabled[derivable_capsE]:
+  assumes "Run (VADeref va sz CAP_PERM_STORE acctype) t vaddr" "trace_assms t"
+    and "0 \<le> sz"
+    and "translate_address (unat vaddr) = Some paddr"
+    and "VA_derivable va s"
+    and "{''PCC''} \<subseteq> accessible_regs s"
+  shows "\<exists>vaddr. access_enabled (run s t) Store vaddr paddr (nat sz) (mem_bytes_of_word data) B0"
+  using assms
+  by (auto intro: VADeref_store_data_enabled)
+
+lemma VADeref_store_data_access_enabled'[derivable_capsE]:
+  assumes "Run (VADeref va sz (perms OR CAP_PERM_STORE) acctype) t vaddr" "trace_assms t"
+    and "0 \<le> sz"
+    and "translate_address (unat vaddr) = Some paddr"
+    and "VA_derivable va s"
+    and "{''PCC''} \<subseteq> accessible_regs s"
+  shows "\<exists>vaddr. access_enabled (run s t) Store vaddr paddr (nat sz) (mem_bytes_of_word data) B0"
+  using assms
+  by (auto intro: VADeref_store_data_enabled')
+
+lemma traces_enabled_bind_VADeref_Let[traces_enabled_combinatorI]:
+  assumes "traces_enabled (VADeref va sz perms acctype \<bind> (\<lambda>addr. f addr y)) s"
+  shows "traces_enabled (VADeref va sz perms acctype \<bind> (\<lambda>addr. let x = y in f addr x)) s"
+  using assms
+  by auto
+
+text \<open>Work around a problem with a common pattern of VirtualAddress dereference
+  in the ASL, where there are two calls to VADeref with the same address and size,
+  but requesting different permissions.  This is used to get the priority of faults
+  right for instructions that both load and store data.  The ASL assumes that the
+  virtual address returned by the two calls is the same, and ignores the second.
+  This does not hold for arbitrary traces, because the returned value depends on
+  register reads, so we'll have to add an assumption on traces that consecutive
+  reads from the same register (without writes in between) read the same values.\<close>
+
+lemma traces_enabled_bind_VADeref_ignore_second[traces_enabled_combinatorI]:
+  assumes "traces_enabled (VADeref va sz perms1 acctype1) s"
+    and "\<And>t1. traces_enabled (VADeref va sz perms2 acctype2) (run s t1)"
+    and "\<And>t1 t2 addr. Run (VADeref va sz (perms1 OR perms2) acctype1) t1 addr \<Longrightarrow> trace_assms t1  \<Longrightarrow> trace_assms t2 \<Longrightarrow> traces_enabled (f addr) (run (run s t1) t2)"
+  shows "traces_enabled (VADeref va sz perms1 acctype1 \<bind> (\<lambda>addr. VADeref va sz perms2 acctype2 \<bind> (\<lambda>_. f addr))) s"
+  sorry
+
+lemma traces_enabled_bind_VADeref_ignore_first[traces_enabled_combinatorI]:
+  assumes "traces_enabled (VADeref va sz perms1 acctype1) s"
+    and "\<And>t1. traces_enabled (VADeref va sz perms2 acctype2) (run s t1)"
+    and "\<And>t1 t2 addr addr'. Run (VADeref va sz perms1 acctype1) t1 addr' \<Longrightarrow> Run (VADeref va sz (perms1 OR perms2) acctype2) t2 addr \<Longrightarrow> trace_assms t1  \<Longrightarrow> trace_assms t2 \<Longrightarrow> traces_enabled (f addr) (run (run s t1) t2)"
+  shows "traces_enabled (VADeref va sz perms1 acctype1 \<bind> (\<lambda>_. VADeref va sz perms2 acctype2 \<bind> (\<lambda>addr. f addr))) s"
+  sorry
 
 end
 
